added or-to-add rewriting; better bounds analysis to assembly checker

src/Assembly/Symbolic.v
@@ -512,6 +512,418 @@ Definition node_beq {A : Set} (arg_eqb : A -> A -> bool) : node A -> node A -> b
 Global Instance reflect_node_beq {A : Set} {arg_eqb} {H : reflect_rel (@eq A) arg_eqb}
   : reflect_rel eq (@node_beq A arg_eqb) | 10 := _.
 
+Compute (node idx).
+Print op. Print symbol.
+
+Definition keep n x := Z.land x (Z.ones (Z.of_N n)).
+
+Compute (keep 5 (-2)).
+
+Print Z.b2z.
+Print negb.
+Print signed.
+
+Compute (signed 1 (0)).
+
+Search signed.
+Compute (keep 4 (-17))%N.
+Compute (-1 / (2^64))%Z. 
+
+Compute (interp_op (fun _ => None) (addcarry 64%N) [2]%Z).
+Compute (interp_op (fun _ => None) (addcarry 64%N) [-2 * (2^64) - 1]%Z).
+
+  
+
+Print fold_right.
+
+Print option_map.
+
+Print interp_op.
+
+Search Z.shiftr.
+
+Compute (Z.shiftr (-1) 5)%Z.
+Check Z.shiftr_div_pow2.
+Print Z.shiftr.
+Print Z.shiftl.
+
+Print fold_right.
+
+Local Open Scope Z_scope.
+
+Definition in_bounds (x : Z) (r : option (Z*Z)) :=
+  match r with
+  | None => True
+  | Some (min, max) => min <= x <= max
+  end.
+
+Ltac inv H := inversion H; subst; clear H.
+
+Definition subset bound1 bound2 := (fst bound2 <=? fst bound1) && (snd bound1 <=? snd bound2).
+
+Definition contains_multiple_of bounds n := fst bounds <=? (snd bounds / n) * n.
+
+Lemma Z_land_ones' : forall (s : N) (a : Z), Z.land a (Z.ones (Z.of_N s)) = (a mod 2 ^ Z.of_N s)%Z.
+Proof. intros. assert (E: Z.le 0 (Z.of_N s)) by lia. auto using Z.land_ones. Qed.
+
+Lemma mod_bounded : forall v s, 0 <= Z.land v (Z.ones (Z.of_N s)) <= Z.ones (Z.of_N s).
+Proof.
+  intros. rewrite Z_land_ones'. cbv [Z.ones]. rewrite Z.shiftl_1_l. assert (H: 2^ Z.of_N s > 0) by lia.
+  apply Z_mod_lt with (a := v) in H. lia.
+Qed.
+
+Lemma div_mul_le x y : 0 < y -> x / y * y <= x.
+Proof.
+  intros H. Search (_ mod _ <= _). assert (H': y <> 0) by lia. apply Z.mod_bound_or with (a := x) in H'.
+  destruct H' as [H'|H'].
+  - rewrite Zmod_eq in H' by lia. destruct H' as [H' _]. lia. 
+  - lia. 
+Qed.
+
+Lemma has_multiple bounds x :
+  0 < x ->
+  contains_multiple_of bounds x = true ->
+  fst bounds <= (snd bounds) / x * x <= snd bounds.
+Proof.
+  destruct bounds as [min max]. cbv [contains_multiple_of]. simpl. intros. Check Z.leb_le. apply Z.leb_le in H0.
+  Compute (1 / 0).
+  split; try assumption. apply div_mul_le. apply H.
+Qed.
+
+Lemma has_no_multiple bounds m :
+  0 < m ->
+  contains_multiple_of bounds m = false ->
+  forall y, 
+  fst bounds <= y <= snd bounds ->
+  ~ (y mod m = 0).
+Proof.
+  intros. intros H'. cbv [contains_multiple_of] in H0. assert (m | y). { apply Znumtheory.Zmod_divide; lia. }
+  cbv [Z.divide] in H2. destruct H2 as [z H2]. clear H'. apply Z.leb_nle in H0.
+  assert (H': y <= snd bounds / m * m \/ snd bounds / m * m < y) by lia. destruct H' as [H'|H'].
+  - apply H0. lia.
+  - subst. assert (snd bounds / m < z). { apply Zmult_lt_reg_r with (p := m); assumption. }
+    clear H0 H'. destruct H1 as [_ H1].
+    Check Z.div_le_mono. remember (Z.div_le_mono _ _ _ H H1) as H1'. clear HeqH1' H1.
+    rewrite Z_div_mult in H1' by lia. lia.
+Qed.
+
+Lemma nondecreasing_max' (a b : Z) (f : Z -> Z) :
+  (forall x, a <= x < b -> f x <= f (x + 1)) ->
+  (forall y, a <= y < b -> f y <= f b).
+Proof.
+  intros. assert (0 <= b - a) by lia. apply Z_of_nat_complete in H1. destruct H1 as [n H1]. assert (b = a + Z.of_nat n) by lia.
+  subst. clear H1. generalize dependent y. induction n as [| n'].
+  - simpl. intros. assert (y = a) by lia. subst. rewrite Z.add_0_r. lia.
+  - intros. destruct (y =? a + Z.of_nat n') eqn: E.
+    + apply Z.eqb_eq in E. subst. rewrite Nat2Z.inj_succ. cbv [Z.succ]. rewrite Z.add_assoc. apply H. apply H0.
+    + apply Z.eqb_neq in E. apply Z.le_trans with (m := f (a + Z.of_nat n')).
+      -- apply IHn'.
+        ++ intros. apply H. lia.
+        ++ lia.
+      -- rewrite Nat2Z.inj_succ. cbv [Z.succ]. rewrite Z.add_assoc. apply H. lia.
+Qed.
+
+Lemma nondecreasing_max (a b : Z) (f : Z -> Z) :
+  (forall x, a <= x < b -> f x <= f (x + 1)) ->
+  (forall y, a <= y <= b -> f y <= f b).
+Proof.
+  intros. destruct (y =? b) eqn:E.
+  - apply Z.eqb_eq in E. subst. lia.
+  - apply Z.eqb_neq in E. apply nondecreasing_max' with (a := a); try lia. apply H.
+Qed.
+
+Lemma nondecreasing_bounds (a b : Z) (f : Z -> Z) :
+  (forall x, a <= x < b -> f x <= f (x + 1)) ->
+  forall y,
+  a <= y <= b ->
+  f a <= f y <= f b.
+Proof.
+  intros. split.
+  - apply nondecreasing_max with (a := a); try lia. intros. apply H. lia.
+  - apply nondecreasing_max with (a := a); try lia. intros. apply H. lia.
+Qed.
+
+(* Lemma nondecreasing_min (a b : Z) (f : Z -> Z) :
+  (forall x, a <= x < b -> f x <= f (x + 1)) ->
+  (forall y, a <= y <= b -> f y <= f b).
+Proof.
+  intros. assert (0 <= b - a) by lia. apply Z_of_nat_complete in H1. destruct H1 as [n H1]. assert (b = a + Z.of_nat n) by lia.
+  subst. clear H1. generalize dependent y. induction n as [| n'].
+  - simpl. intros. assert (y = a) by lia. subst. rewrite Z.add_0_r. lia.
+  - intros. destruct (y =? a + Z.of_nat n') eqn: E.
+    + apply Z.eqb_eq in E. subst. rewrite Nat2Z.inj_succ. cbv [Z.succ]. rewrite Z.add_assoc. apply H. apply H0.
+    + apply Z.eqb_neq in E. apply Z.le_trans with (m := f (a + Z.of_nat n')).
+      -- apply IHn'.
+        ++ intros. apply H. lia.
+        ++ lia.
+      -- rewrite Nat2Z.inj_succ. cbv [Z.succ]. rewrite Z.add_assoc. apply H. lia.
+Qed. *)
+
+(* Lemma nondecreasing_min (a b : Z) (f : Z -> Z) :
+  (forall x, a <= x < b -> f x <= f (x + 1)) ->
+  (forall y, a <= y <= b -> f a <= f y).
+Proof.
+  intros. remember (fun x => - (f (a + b - x))) as g. assert (g (a + b - y) <= g (b)).
+  - apply nondecreasing_max with (a := a); try lia. intros. subst. assert (f (a + b - (x + 1)) <= (f (a + b - x))).
+    + replace (a + b - x) with (a + b - (x + 1) + 1) by lia. apply H. lia.
+    + lia.
+  - subst. replace (a + b - b) with a in H1 by lia. replace (a + b - (a + b - y)) with y in H1 by lia. lia.
+Qed. *)
+
+Lemma mod_nondecreasing (a b : Z) :
+  b > 0 ->
+  ~ ((a + 1) mod b = 0) ->
+  a mod b <= (a + 1) mod b.
+Proof.
+  intros. rewrite PullPush.Z.add_mod_l.
+  assert (H': 0 <= a mod b + 1 < b).
+  - Check Z.mod_pos_bound. assert (0 <= a mod b < b). { apply Z.mod_pos_bound. lia. }
+    split; try lia. destruct (a mod b =? b - 1) eqn:E.
+    + apply Z.eqb_eq in E. rewrite PullPush.Z.add_mod_l in H0. rewrite E in H0. simpl in H0. replace (b - 1 + 1) with (b) in H0 by lia.
+      apply Z_mod_same in H. exfalso. auto.
+    + apply Z.eqb_neq in E. lia.
+  - Check Z.mod_small. apply Z.mod_small in H'. rewrite H'. lia.
+Qed.
+
+Lemma no_multiple_bounds lower upper m :
+  0 < m ->
+  contains_multiple_of (lower + 1, upper) m = false ->
+  forall x,
+  lower <= x <= upper ->
+  lower mod m <= x mod m <= upper mod m.
+Proof.
+  intros. remember (fun x => x mod m) as f. assert (forall x, f x = x mod m). { rewrite Heqf. reflexivity. }
+  repeat rewrite <- H2. clear H2. apply nondecreasing_bounds with (a := lower); try lia.
+    intros. subst. apply mod_nondecreasing; try lia. apply has_no_multiple with (bounds := (lower + 1, upper)); try lia.
+  - assumption.
+  - simpl. lia.
+Qed.
+
+(* Lemma no_multiple_min_left bounds m :
+  0 < m ->
+  contains_multiple_of bounds m = false ->
+  forall x,
+  fst bounds <= x <= snd bounds ->
+  (fst bounds) mod m <= x mod m.
+Proof.
+  intros. remember (fun x => x mod m) as f. assert (forall x, f x = x mod m). { rewrite Heqf. reflexivity. }
+  repeat rewrite <- H2. clear H2. apply nondecreasing_max with (a := fst bounds); try lia.
+    intros. subst. apply mod_nondecreasing; try lia. apply has_no_multiple with (bounds := bounds); try lia.
+    assumption.
+Qed. *)
+
+Definition bounds_modulo Z_bounds modulus :=
+ if contains_multiple_of (fst Z_bounds + 1, snd Z_bounds) modulus then 
+   (0, modulus - 1) 
+  else
+   (fst Z_bounds mod modulus, snd Z_bounds mod modulus).
+
+Lemma bounds_modulo_bounds b m x :
+  0 < m ->
+  in_bounds x (Some b) ->
+  in_bounds (x mod m) (Some (bounds_modulo b m)).
+Proof.
+  simpl. destruct b as [min max]. intros. destruct (bounds_modulo (min, max) m) as [min' max'] eqn:E.
+  cbv [bounds_modulo] in E. simpl in E. destruct (contains_multiple_of (min + 1, max) m) eqn:E'.
+  - inv E. Search (0 <= _ mod _). apply Z.mod_pos_bound with (a := x) in H. lia.
+  - inv E. apply no_multiple_bounds; try lia. assumption.
+Qed.
+
+Definition plain_arg_bounds arg_bounds : option (list (Z*Z)) :=
+  fold_right (fun maybe_bound result =>
+                  match maybe_bound, result with
+                  | Some bound, Some bounds => Some (bound :: bounds)
+                  | _, None => None
+                  | None, _ => None
+                  end) (Some []) arg_bounds.
+
+Lemma plain_bounds_bound :
+  forall args arg_bounds plain_bounds,
+  plain_arg_bounds arg_bounds = Some plain_bounds ->
+  Forall2 in_bounds args arg_bounds ->
+  Forall2 in_bounds args (map Some plain_bounds).
+Proof.
+  intros args. induction args as [| arg args' IHargs'].
+  - intros. inv H0. inv H. constructor.
+  - intros. inv H0. rename y into arg_bound. rename l' into arg_bounds'. simpl in H.
+    destruct arg_bound as [plain_bound|]; destruct (plain_arg_bounds arg_bounds') as [plain_bounds'|] eqn:E.
+    + inv H. rewrite map_cons. constructor; try assumption. apply IHargs' with (arg_bounds := arg_bounds');
+      assumption.
+    + discriminate H.
+    + discriminate H.
+    + discriminate H.
+Qed.
+
+Definition accumulate (f : Z -> Z -> Z) (a0 : Z*Z) (args : list (Z*Z)) : Z*Z :=
+  fold_right (fun bound bound' => (f (fst bound) (fst bound'), f (snd bound) (snd bound'))) a0 args.
+
+Lemma sum_bounded plain_bounds:
+  forall args : list Z,
+  Forall2 in_bounds args (map Some plain_bounds) ->
+  in_bounds (fold_right Z.add 0 args) (Some (accumulate Z.add (0, 0) plain_bounds)).
+Proof.
+  induction plain_bounds as [| pb pbs'].
+  - intros. inv H. simpl. lia.
+  - intros. rewrite map_cons in H. inv H. rename x into arg. rename l into args'. apply IHpbs' in H4.
+    clear IHpbs'. simpl in *. destruct pb as [min1 max1]. destruct (accumulate _ _ pbs') as [min2 max2]. simpl. lia.
+Qed.
+
+(* Lemma product_bounded plain_bounds:
+  forall args : list Z,
+  Forall2 in_bounds args (map Some plain_bounds) ->
+  in_bounds (fold_right Z.mul 0 args) (Some (accumulate Z.mul (0, 0) plain_bounds)).
+Proof.
+  induction plain_bounds as [| pb pbs'].
+  - intros. inv H. simpl. lia.
+  - intros. rewrite map_cons in H. inv H. rename x into arg. rename l into args'. apply IHpbs' in H4.
+    clear IHpbs'. simpl in *. destruct pb as [min1 max1]. destruct (accumulate _ _ pbs') as [min2 max2]. simpl. lia.
+Qed. *)
+
+Definition bounds_positive (plain_bounds : list (Z*Z)) :=
+  fold_right (fun bound pos_so_far => (0 <=? fst bound) && pos_so_far) true plain_bounds.
+
+Lemma pos_prod_pos bounds :
+  bounds_positive bounds = true ->
+  0 <= fst (accumulate Z.mul (1, 1) bounds).
+Proof.
+  induction bounds as [|bound bounds'].
+  - intros. simpl. lia.
+  - intros. simpl in H. apply andb_prop in H. destruct H as [H1 H2]. apply IHbounds' in H2. apply Z.leb_le in H1.
+    simpl. lia.
+Qed.
+
+(* Lemma mul_le_mono_double a1 a2 b1 b2 :
+  0 <= a1 -> 
+  0 <= a2 -> 
+  a1 <= b1 ->
+  a2 <= b2 -> 
+  a1 * a2 <= b1 * b2.
+Proof.
+  intros. apply Z.le_trans with (m := a1 * b2).
+  - Search (_ * _ <= _ * _). apply Z.mul_le_mono_nonneg_l; lia.
+  -  *)
+
+Lemma product_bounded plain_bounds:
+  bounds_positive plain_bounds = true ->
+  forall args : list Z,
+  Forall2 in_bounds args (map Some plain_bounds) ->
+  in_bounds (fold_right Z.mul 1 args) (Some (accumulate Z.mul (1, 1) plain_bounds)).
+Proof.
+  induction plain_bounds as [| pb pbs'].
+  - intros. inv H0. simpl. lia.
+  - intros. rewrite map_cons in H0. inv H0. rename x into arg. rename l into args'. simpl in H.
+    apply andb_prop in H. destruct H as [H1 H2]. apply Z.leb_le in H1. 
+    apply (IHpbs' H2) in H5. clear IHpbs'. simpl in H5. simpl in H4. destruct pb as [min1 max1]. simpl. 
+    apply pos_prod_pos in H2. simpl in *. destruct (accumulate _ _ pbs') as [min2 max2]. simpl in *.
+    split.
+    + apply Z.le_trans with (m := arg * min2).
+      -- apply Z.mul_le_mono_nonneg_r; lia.
+      -- apply Z.mul_le_mono_nonneg_l; lia.
+    + apply Z.le_trans with (m := arg * max2).
+      -- apply Z.mul_le_mono_nonneg_l; lia.
+      -- apply Z.mul_le_mono_nonneg_r; lia.
+Qed.
+
+(* input bounds should be nonnegative.  if lower bound is less than zero, returns None *)
+Definition bound_node (o : op) (arg_bounds : list (option (Z*Z))) : option (Z*Z) :=
+  match o, (plain_arg_bounds arg_bounds) with
+  | old s _, Some nil => Some (0, Z.ones (Z.of_N s))
+  | const n, Some nil => Some (n, n)
+  | add s, Some actual_bounds =>  let Z_bounds := (accumulate Z.add (0, 0) actual_bounds) in Some (bounds_modulo Z_bounds (2 ^ (Z.of_N s)))
+  | addcarry s, Some actual_bounds => let addZ_bounds := accumulate Z.add (0, 0) actual_bounds in
+                                      if subset addZ_bounds (0, Z.ones (Z.of_N s)) then Some (0, 0) else Some (0, 1)
+  | addcarry s, None => Some (0, 1)
+  | shr s, Some [a; b] => if (0 <=? fst a) && (0 <=? fst b) then
+                            let Z_bounds := (Z.shiftr (fst a) (snd b), Z.shiftr (snd a) (fst b)) in Some (bounds_modulo Z_bounds (2 ^ (Z.of_N s)))
+                          else
+                            Some (0, Z.ones (Z.of_N s))
+  | mul s, Some actual_bounds =>  if bounds_positive actual_bounds then
+                                    let Z_bounds := accumulate Z.mul (1, 1) actual_bounds in Some (bounds_modulo Z_bounds (2 ^ Z.of_N s))
+                                  else
+                                    Some (0, Z.ones (Z.of_N s))
+  | slice lo sz, Some [a] => let Z_bounds := (Z.shiftr (fst a) (Z.of_N lo), Z.shiftr (snd a) (Z.of_N lo)) in Some (bounds_modulo Z_bounds (2 ^ Z.of_N sz))
+  | addZ, Some actual_bounds => Some (accumulate Z.add (0, 0) actual_bounds)
+  | mulZ, Some actual_bounds => if bounds_positive actual_bounds then
+                                  Some (accumulate Z.mul (1, 1) actual_bounds)
+                                else
+                                  None
+  | (old s _ | slice _ s | mul s | shl s | shr s | sar s | neg s | and s | or s | xor s), _ => Some (0, Z.ones (Z.of_N s))
+  | _, _ => None
+  end.
+
+Ltac thing:= match goal with
+  | H : Forall2 _ _ _ |- _ => inversion H; clear H; subst
+  end.
+
+Lemma interp_bound_node ctx o args arg_bounds n :
+  Forall2 in_bounds args arg_bounds ->
+  interp_op ctx o args = Some n ->
+  in_bounds n (bound_node o arg_bounds).
+Proof.
+  intros H1 H2. destruct (plain_arg_bounds arg_bounds) as [plain_bounds|] eqn:E.
+  - remember (plain_bounds_bound _ _ _ E H1) as H_p. clear HeqH_p. cbv [bound_node]. rewrite E. simpl.
+    clear H1 E arg_bounds. destruct o eqn:Eo; try apply I; simpl in H2; try (inv H2; apply mod_bounded);
+    try (destruct args as [| arg1 args1]; try destruct args1 as [| arg2 args2]; try destruct args2 as [| arg3 args3]; inv H2; apply mod_bounded).
+    + (* o = old s s0 *)
+      destruct args as [| arg args']; try discriminate H2. destruct plain_bounds as [|pb pbs']; try apply I; try apply mod_bounded.
+      -- destruct (ctx s0) as [v|]; try discriminate H2. inv H2. simpl. apply mod_bounded.
+      -- destruct (ctx s0) as [v|]; try discriminate H2. inv H2. simpl. apply mod_bounded.
+    + (* o = const z *)
+      destruct args as [| arg args']; try discriminate H2. destruct plain_bounds as [|pb pbs']; try apply I. inv H2. simpl. lia.
+    + (* o = add s *)
+      inv H2. rewrite Z_land_ones'. apply bounds_modulo_bounds; try lia. apply sum_bounded. assumption.
+    + (* o = addcarry s *)
+      destruct (subset _ _) eqn:E.
+      -- simpl. assert (n = 0); try lia. inv H2. rewrite Z.shiftr_div_pow2; try lia.
+         replace (_ / _) with 0; try apply Zmod_0_l. symmetry. apply Zdiv_small.
+         apply sum_bounded in H_p. destruct (accumulate _ _ _) as [min max]. cbv [subset] in E. simpl in *.
+         apply andb_prop in E. destruct E as [E1 E2].
+         apply Z.leb_le in E1. apply Z.leb_le in E2. cbv [Z.ones] in E2. rewrite Z.shiftl_1_l in E2. lia.
+      -- clear E H_p plain_bounds. simpl. assert (0 <= n < 2); try lia. inv H2. apply Z.mod_pos_bound. lia.
+    + (* o = shr s *)
+      destruct plain_bounds as [| pb1 [| pb2 [| pbs'] ] ].
+      -- inv H_p. congruence.
+      -- inv H_p. inv H4. congruence.
+      -- inv H_p. inv H4. inv H6. inv H2. rewrite Z_land_ones'. destruct (_ && _) eqn:E.
+        ++ apply bounds_modulo_bounds; try lia. apply andb_prop in E. destruct E as [E1 E2]. apply Z.leb_le in E1.
+           apply Z.leb_le in E2. simpl in *. destruct pb1 as [min1 max1]. destruct pb2 as [min2 max2]. simpl in *.
+           repeat rewrite Z.shiftr_div_pow2 by lia. split.
+          --- Check Z.le_trans. apply Z.le_trans with (m := min1 / 2 ^ x0).
+            +++ apply Z.div_le_compat_l; try lia. split; try lia.
+              apply Z.pow_le_mono_r; lia.
+            +++ apply Z.div_le_mono; lia.
+          --- apply Z.le_trans with (m := x / 2 ^ min2).
+            +++ apply Z.div_le_compat_l; try lia. split; try lia. apply Z.pow_le_mono_r; lia.
+            +++ apply Z.div_le_mono; lia.
+        ++ clear H3 H5 E. simpl. rewrite <- Z_land_ones'. apply mod_bounded.
+      -- inv H_p. inv H4. inv H6. congruence.
+    + (* o = slice lo sz *)
+      destruct plain_bounds as [| pb1 [| pb2 pbs'] ].
+      -- repeat thing. congruence.
+      -- repeat thing. inv H2.
+          rewrite Z_land_ones'. apply bounds_modulo_bounds; try lia. simpl. repeat rewrite Z.shiftr_div_pow2 by lia.
+          simpl in H3. destruct pb1 as [min max]. simpl. split.
+        ++ apply Z.div_le_mono; lia.
+        ++ apply Z.div_le_mono; lia.
+      -- repeat (thing; try congruence). 
+    + (* o = mul s *)
+      destruct (bounds_positive plain_bounds) eqn:E.
+      -- inv H2. rewrite Z_land_ones'. apply bounds_modulo_bounds; try lia. simpl. apply product_bounded; assumption.
+      -- simpl. inv H2. apply mod_bounded.
+    + (* o = addZ *) simpl. inv H2. apply sum_bounded; assumption.
+    + (* o = mulZ *) destruct (bounds_positive plain_bounds) eqn:E; try apply I. simpl. inv H2. apply product_bounded; assumption.
+  - simpl in E. cbv [bound_node]. rewrite E.
+    destruct o eqn:Eo; try apply I. 
+    all: destruct args as [| arg1 [| arg2 [| arg3 args3] ] ]; try (inv H2; apply mod_bounded). 
+    all: try (simpl in H2; destruct (ctx s0); inv H2; apply mod_bounded).
+    all: try (simpl; assert (0 <= n < 2); try lia; inv H2; apply Z.mod_pos_bound; lia).
+    + (* and s *) cbv [interp_op] in H2. rewrite Z.land_m1'_l in H2. inv H2. simpl. cbv [Z.ones]. repeat rewrite Z.shiftl_1_l. lia.
+    + (* or s *) cbv [interp_op] in H2. simpl in H2. inv H2. simpl.  cbv [Z.ones]. repeat rewrite Z.shiftl_1_l. lia.
+    + (* xor s *) cbv [interp_op] in H2. simpl in H2. inv H2. simpl.  cbv [Z.ones]. repeat rewrite Z.shiftl_1_l. lia.
+    + (* mul s *) cbv [interp_op] in H2. rewrite Z_land_ones' in H2. inv H2. simpl. cbv [Z.ones]. rewrite Z.shiftl_1_l.
+      assert (0 <= 1 mod 2^Z.of_N s < 2 ^ Z.of_N s); try lia. apply Z.mod_bound_pos; lia.
+Qed.
+
 Class description := descr : option ((unit -> string) * bool (* always show *)).
 Typeclasses Opaque description.
 Definition eager_description := option (string * bool).
@@ -526,13 +938,18 @@ Existing Class node_ok.
 Hint Extern 1 (node_ok ?i ?n) => exact (@new_node_ok n I i) : typeclass_instances.
 Module Old.
 Module dag.
-  Definition t : Type := list (node idx * description).
+  Definition t : Type := list (node idx * description * (option (Z*Z))).
   Definition empty : t := nil.
   Definition size (d : t) : N := N.of_nat (List.length d).
   Definition lookup (d : t) (i : idx) : option (node idx)
-    := option_map fst (List.nth_error d (N.to_nat i)).
+    := option_map (fun x => fst (fst x)) (List.nth_error d (N.to_nat i)).
+  Definition lookup_bounds (d : t) (i : idx) : option (Z*Z)
+    :=  match (List.nth_error d (N.to_nat i)) with
+        | Some thing => snd thing
+        | None => None
+        end.
   Definition reverse_lookup (d : t) (i : node idx) : option idx
-    := option_map N.of_nat (List.indexof (fun '(n', _) => node_beq N.eqb i n') d).
+    := option_map N.of_nat (List.indexof (fun '(n', _, _) => node_beq N.eqb i n') d).
   Definition size_ok (d : t) : Prop
     := True.
   Definition all_nodes_ok (d : t) : Prop
@@ -545,7 +962,7 @@ Module dag.
     := match reverse_lookup d n with
        | Some i => (i, d)
        | None
-         => (size d, d ++ [(n, descr)])
+         => (size d, d ++ [(n, descr, bound_node (fst n) (map (lookup_bounds d) (snd n)))])
        end.
   Definition gensym (s:OperationSize) (d : t) : node idx
     := (old s (size d), []).
@@ -560,12 +977,12 @@ Module dag.
     := option_map (fun '(descr, always_show) => (descr tt, always_show)).
 
   Module eager.
-    Definition t := list (idx * node idx * eager_description).
+    Definition t := list (idx * node idx * eager_description * option (Z*Z)).
     Definition force (d : dag.t) : eager.t
-      := List.map (fun '(idx, (n, descr)) => (N.of_nat idx, n, force_description descr))
+      := List.map (fun '(idx, (n, descr, bounds)) => (N.of_nat idx, n, force_description descr, bounds))
                   (List.enumerate d).
     Definition description_lookup (d : eager.t) (descr : string) : list idx
-      := List.map (fun '(idx, _, _) => idx) (List.filter (fun '(_, _, descr') => match get_eager_description_description descr' with Some descr' => String.eqb descr descr' | _ => false end) d).
+      := List.map (fun '(idx, _, _, _) => idx) (List.filter (fun '(_, _, descr', _) => match get_eager_description_description descr' with Some descr' => String.eqb descr descr' | _ => false end) d).
   End eager.
 
   Definition M T := t -> T * t.
@@ -621,6 +1038,8 @@ Module dag.
                      | [ H : nth_error (_ :: _) ?x = _ |- _ ] => destruct x eqn:?; cbn [nth_error] in H
                      end ].
   Qed.
+
+Check dag.reverse_lookup.
 
   Lemma reverse_lookup_merge_node {d : t}
         {ok : ok d} {descr : description} (n n' : node idx)
@@ -1335,8 +1754,6 @@ Ltac t:= match goal with
   | _ => progress subst
   end.
 
-Ltac inv H := inversion H; subst; clear H.
-
 Lemma bound_sum' G d
   es (He : Forall (fun e => forall b, bound_expr e = Some b ->
        forall (d : dag) (v : Z), eval G d e v -> (0 <= v <= b)%Z) es)
@@ -1467,9 +1884,12 @@ Proof.
   - apply permute_commutative with (args := args'); assumption.
 Qed.
 
+Check eval.
+
+Definition bounds_ok (d : dag) := forall G i n, eval G d (ExprRef i) n -> in_bounds n (dag.lookup_bounds d i).
 (* the gensym state cannot map anything past the end of the dag *)
 Definition gensym_ok (G : symbol -> option Z) (d : dag) := forall s _v, G s = Some _v -> (s < dag.size d)%N.
-Definition dag_ok G (d : dag) := dag.ok d /\ dag.all_nodes_ok d /\ forall i r, dag.lookup d i = Some r -> exists v, eval G d (ExprRef i) v.
+Definition dag_ok G (d : dag) := bounds_ok d /\ dag.ok d /\ dag.all_nodes_ok d /\ forall i r, dag.lookup d i = Some r -> exists v, eval G d (ExprRef i) v.
 Definition gensym_dag_ok G d := gensym_ok G d /\ dag_ok G d.
 
 Lemma gensym_ok_size_Proper G d1 d2
@@ -1486,7 +1906,275 @@ Proof using Type.
   cbv [gensym_dag_ok dag_ok gensym_ok].
   repeat match goal with |- _ /\ _ => split end; try exact _; intros *;
     rewrite ?dag.lookup_empty; try congruence.
+
+  cbv [bounds_ok]. intros. inv H. rewrite dag.lookup_empty in H1. discriminate H1.
 Qed.
+
+Check nth_error_app.
+Check dag.lookup_bounds.
+Check dag.size.
+Check dag.lookup_bounds.
+
+Lemma split_lookup_bounds d1 d2 i : 
+  dag.lookup_bounds (d1 ++ d2) i = if N.ltb i (dag.size d1) then dag.lookup_bounds d1 i else dag.lookup_bounds d2 (i - dag.size d1)%N.
+Proof.
+  destruct (i <? dag.size d1)%N eqn:E. 
+  - cbv [dag.lookup_bounds]. rewrite nth_error_app. destruct (lt_dec _ _).
+    + reflexivity.
+    + apply N.ltb_lt in E. exfalso. apply n. cbv [dag.size] in E. lia.
+  - cbv [dag.lookup_bounds]. rewrite nth_error_app. destruct (lt_dec _ _).
+    + apply N.ltb_nlt in E. exfalso. apply E. cbv [dag.size]. lia.
+    + cbv [dag.size]. replace (N.to_nat (i - N.of_nat (Datatypes.length d1))) with (N.to_nat i - Datatypes.length d1)%nat by lia. reflexivity.
+Qed.
+
+Lemma split_lookup d1 d2 i : 
+  dag.lookup (d1 ++ d2) i = if N.ltb i (dag.size d1) then dag.lookup d1 i else dag.lookup d2 (i - dag.size d1)%N.
+Proof.
+  destruct (i <? dag.size d1)%N eqn:E. 
+  - cbv [dag.lookup]. rewrite nth_error_app. destruct (lt_dec _ _).
+    + reflexivity.
+    + apply N.ltb_lt in E. exfalso. apply n. cbv [dag.size] in E. lia.
+  - cbv [dag.lookup]. rewrite nth_error_app. destruct (lt_dec _ _).
+    + apply N.ltb_nlt in E. exfalso. apply E. cbv [dag.size]. lia.
+    + cbv [dag.size]. replace (N.to_nat (i - N.of_nat (Datatypes.length d1))) with (N.to_nat i - Datatypes.length d1)%nat by lia. reflexivity.
+Qed.
+
+Lemma something ctx G d1 d2 i v n0 :
+  eval ctx d1 (ExprRef i) v ->
+  eval G (d1 ++ d2) (ExprRef i) n0 ->
+  eval G d1 (ExprRef i) n0.
+Proof.
+  intros. generalize dependent n0. remember (ExprRef i) as e. generalize dependent i. induction H.
+  - intros. inv H2. rewrite split_lookup in H4. destruct (i <? dag.size d1)%N eqn:E.
+    + rewrite H4 in H. clear E. inv H. apply ERef with (op := op0) (args := args) (args' := args'0).
+      -- apply H4.
+      -- clear H4 H1 H6. generalize dependent args'. generalize dependent args'0. induction args as [| arg morargs IHmorargs].
+        ++ intros. inv H5. constructor.
+        ++ intros. simpl in *. inv H5. inv H0. destruct H3 as [H3 H5]. constructor.
+          --- apply H5 with (i := arg); try reflexivity. apply H2.
+          --- apply IHmorargs with (args' := l'0).
+            +++ assumption.
+            +++ assumption.
+      -- assumption.
+    + exfalso. clear H0 H1 H4 H5 H6 n0 op1 args0 args'0. cbv [dag.lookup] in H. destruct (nth_error _ _) as [sth|] eqn:E'.
+      -- clear H. apply N.ltb_nlt in E. apply E; clear E. cbv [dag.size]. apply nth_error_value_length in E'.
+         lia.
+      -- discriminate.
+  - intros. discriminate Heqe.
+Qed.
+
+Lemma much_something ctx d1 d2 args' args G :
+  (forall (i : idx) (r : node idx), dag.lookup d1 i = Some r -> exists v : Z, eval ctx d1 (ExprRef i) v) ->
+  Forall (fun j : N => (j < dag.size d1)%N) args ->
+  Forall2 (eval G (d1 ++ d2)) (map ExprRef args) args' ->
+  Forall2 (eval G d1) (map ExprRef args) args'.
+Proof.
+  intros. generalize dependent args'. induction args as [| arg args1 IHargs1].
+  - intros. inv H1. constructor.
+  - intros. inv H0. inv H1. constructor.
+    + clear IHargs1 H7 H5. remember H3 as H3'; clear HeqH3'. inv H3. rewrite split_lookup in H1. 
+      destruct (arg <? dag.size d1)%N eqn:E.
+      -- clear E H4. apply H in H1. clear H. destruct H1 as [v H1]. apply something with (ctx := ctx) (d2 := d2) (v := v); assumption.
+      -- exfalso. apply N.ltb_nlt in E. apply E. apply H4.
+    + apply IHargs1; assumption.
+Qed.
+
+Print dag.merge_node.
+
+Lemma node_doesnt_reference_self G d o args i n :
+  eval G d (ExprRef i) n ->
+  dag.lookup d i = Some (o, args) ->
+  Forall (fun j => j <> i) args.
+Proof.
+  intros. remember (ExprRef i) as e. rewrite Forall_Exists_neg. intros H3. induction H.
+  - inv Heqe. rewrite H0 in H. inv H. clear H0.
+    assert (H4: forall a b, (fun (e : expr) (n : Z) => eval G d e n /\ (e = ExprRef i -> False)) a b ->
+                            (fun (e : expr) (n : Z) => (e = ExprRef i -> False)) a b) by intuition.
+    apply (Forall2_weaken H4) in H1. clear H4. apply Forall2_Forall_ignore_l in H1. destruct H1 as [_ H1].
+    apply Exists_exists in H3. rewrite Forall_map in H1. rewrite Forall_forall in H1. destruct H3 as [x [H3 H4] ].
+    apply H1 with (x := x).
+    + assumption.
+    + f_equal. assumption.
+  - discriminate Heqe.
+Qed.
+
+Lemma args_in_bounds G d o args i n :
+  eval G d (ExprRef i) n ->
+  dag.lookup d i = Some (o, args) ->
+  Forall (fun j => N.lt j (dag.size d)) args.
+Proof.
+  intros. inv H. rewrite H0 in H2. inv H2. clear H0 H4. generalize dependent args'.
+  induction args0 as [| arg0 args0' IHargs0'].
+  - constructor.
+  - intros. inv H3. constructor.
+    + inv H1. cbv [dag.size]. assert (N.to_nat arg0 < Datatypes.length d)%nat; try lia. cbv [dag.lookup] in H0.
+      destruct (nth_error _ _) as [sth|] eqn:E; try discriminate H0. clear H0. apply nth_error_value_length with (x := sth).
+      assumption.
+    + apply IHargs0' with (args' := l'). apply H4.
+Qed.
+
+(* Lemma in_bounds_and_not_self G d i n :
+  eval G d (ExprRef i) n ->
+  exists o args,
+  dag.lookup d i = Some (o, args) /\
+  Forall (fun j => N.lt j (dag.size d - 1)) args. *)
+
+
+
+Print dag_ok.
+Print dag.ok.
+Print dag.all_nodes_ok.
+Print node_ok.
+
+
+(* Lemma eval_args_in_range G d o args descr bound n :
+  eval G (d ++ [((o, args), descr, bound)]) (ExprRef (dag.size d)) n ->
+  Forall (fun j => N.lt j (dag.size d)) args.
+Proof.
+  intros. remember (ExprRef (dag.size d)) as e.
+  apply Forall_impl with (P := fun j => ~ (j = dag.size d) /\ ~ (dag.size d < j)%N).
+  - lia.
+  - apply Forall_and.
+    + rewrite Forall_Exists_neg. induction H.
+      -- inv Heqe. inv H. rewrite split_lookup in H3. rewrite N.ltb_irrefl in H3. rewrite N.sub_diag in H3. inv H3.
+         intros H. Search Exists. remember H as H'; clear HeqH'. apply Exists_exists in H'. Search Forall2. Check Forall2_weaken.
+         assert (H2: forall a b, (fun (e : expr) (n : Z) => eval G (d ++ [(op0, args0, descr, bound)]) e n /\ (e = ExprRef (dag.size d) -> ~ Exists (fun x : N => x = dag.size d) args0)) a b -> 
+                             (fun (e : expr) (n : Z) => (e = ExprRef (dag.size d) -> ~ Exists (fun x : N => x = dag.size d) args0)) a b) by intuition.
+         apply (Forall2_weaken H2) in H0. clear H2. apply Forall2_Forall_ignore_l in H0. destruct H0 as [_ H0].
+         Check Forall_map. rewrite Forall_map in H0. rewrite Forall_forall in H0.
+         destruct H' as [x [H1' H2'] ]. cbv [not] in H0. apply H0 with (x := x); try assumption. f_equal. assumption.
+      -- discriminate Heqe.
+    + subst. inv H. clear H2 H3. cbv [dag.lookup] in H1. destruct (nth_error _ _) as [sth|] eqn:E; try discriminate H1.
+      clear H1. Search nth_error. apply nth_error_value_length in E.
+         { eapply Forall2_weaken. Check Forall_impl. Check Forall2_weaken. with (P := fun (e : expr) (n : Z) => eval G (d ++ [(op0, args0, descr, bound)]) e n /\ (e = ExprRef (dag.size d) -> ~ Exists (fun x : N => x = dag.size d) args0)).
+
+
+
+  Check Forall2_weaken.
+         apply Forall2_weaken in H0. with (Q := fun e n => (e = ExprRef (dag.size d) -> ~ Exists (fun x : N => x = dag.size d) args0)) in H0.
+
+
+
+
+
+
+         induction args0 as [| arg0 args0' IHargs0'].
+        ++ intros H. inv H.
+        ++ intros H. inv H.
+          --- apply IHargs0' in H0.
+    + inv H0. clear H5 H1. destruct H3 as [_ H3]. constructor.
+      -- 
+
+
+
+  apply Forall_impl with (P := fun j => ~ (j = dag.size d) /\ ~ (dag.size d <= j)%N).
+  - lia.
+  - apply Forall_and.
+    + rewrite Forall_Exists_neg. induction H'.
+      -- 
+ induction H'. 2: {
+  -  *)
+  
+
+
+Lemma merge_node_bounds_ok {descr : description} ctx d n : 
+  dag_ok ctx d ->
+  bounds_ok (snd (dag.merge_node n d)).
+Proof.
+  intros. cbv [dag_ok] in H. destruct H as [H1 [_ [_ H2] ] ]. Check eval_weaken_merge_node.
+  cbv [bounds_ok] in *. intros. destruct n as [o args].
+  remember (dag.merge_node (o, args) d) as i_d'. Check eval_weaken_merge_node. cbv [dag.merge_node] in Heqi_d'. 
+  destruct (dag.reverse_lookup _ _) as [new_i|].
+  - subst. simpl in *. apply H1 with (G := G). apply H.
+  - subst. simpl in *. remember H as H'; clear HeqH'. inv H. rewrite split_lookup_bounds. remember H3 as H3'; clear HeqH3'.
+    rewrite split_lookup in H3.
+    destruct (i <? dag.size d)%N eqn:E'.
+    + remember (H2 _ _ H3) as H6; clear HeqH6 H2. destruct H6 as [v H6]. apply (something _ _ _ _ _ _ _ H6) in H'.
+      apply H1 with (G := G). apply H'.
+    + remember (map _ _) as no. cbv [dag.lookup_bounds]. subst. cbv [dag.lookup] in H3.
+      destruct (N.to_nat _) as [| [| n''] ] eqn:E''; try discriminate H3. simpl in H3. simpl. inv H3. Check interp_bound_node.
+      (* destruct (bound_node _ _) as [ [min max]|]; try apply I.  *)apply N.ltb_nlt in E'. assert (E1'': i = dag.size d) by lia.
+      clear E' E''. subst. remember H' as H''; clear HeqH''. inv H'. rewrite H0 in H3'. inv H3'. clear H3 H6. Check node_doesnt_reference_self.
+      remember (node_doesnt_reference_self _ _ _ _ _ _ H'' H0) as H3; clear HeqH3.
+      remember (args_in_bounds _ _ _ _ _ _ H'' H0) as H6; clear HeqH6.
+      assert (E: Forall (fun j : N => N.lt j (dag.size d)) args0).
+      { rewrite Forall_forall in H3. rewrite Forall_forall in H6. rewrite Forall_forall. intros.
+        remember (H3 _ H) as H7; clear HeqH7. apply H6 in H. cbv [dag.size] in H. Search Datatypes.length.
+        rewrite app_length in H. simpl in H. cbv [dag.size] in H7. cbv [dag.size]. clear H4 H5 H'' H0 H3 H6. lia. }
+      apply (much_something _ _ _ _ _ _ H2 E) in H4.
+      Check interp_bound_node. apply interp_bound_node with (ctx := G) (args := args').
+      -- clear H2 E H5 H3 H6 H0 H''. generalize dependent args'. induction args0 as [| arg0 args0' IHargs0'].
+        ++ intros. inv H4. constructor.
+        ++ intros. inv H4. constructor.
+          --- apply H1 with (G := G). apply H2.
+          --- apply IHargs0'. apply H5.
+      -- assumption.
+Qed.
+    
+
+(*
+remember (ExprRef i) as e. generalize dependent i.
+    induction H.
+    + intros. inv Heqe. rewrite split_lookup_bounds. rewrite split_lookup in H.
+      destruct (i0 <? dag.size d)%N.
+      -- Check interp_bound_node. remember (H2 _ _ H) as H4; clear HeqH4.
+
+
+apply H with (G := G). assert (dag_ok G d). { fail. }
+         destruct H3. destruct H4. destruct H5.
+
+
+
+
+
+
+ inv H0. rewrite split_lookup in H2. destruct (i <? dag.size d)%N eqn:E.
+    {+ destruct (dag.lookup_bounds d i) as [bound|] eqn:E1; try apply I. simpl. remember (bounds_in_range _ _ _ _ _ E1 H2) as H2'. clear HeqH2'.
+      assert (Forall2 (eval G d) (map ExprRef args0) args'). { reflexivity. }
+      clear H3. rewrite <- E1. apply H with (G := G). apply ERef with (op := op0) (args := args0) (args' := args'); assumption.
+    + cbv [dag.lookup] in H2. remember (dag.lookup_bounds d) as dontexpand. cbv [dag.lookup_bounds]. subst. destruct (N.to_nat _) as [| [| n''] ]; try discriminate H2. simpl in H2. } 
+      inv H2. simpl. assert ( cbv [nth_error] in H2. simpl in H2. try discriminate H2. cbv [nth_error] in H2.
+ 
+
+
+
+
+
+
+
+remember ([(o, args, _, _)]) as d2. inv Heqi_d'. clear H1. simpl in *. remember H0 as H0'; clear HeqH0'. inv H0. remember (d ++ _) as d'. cbv [dag.lookup_bounds].
+    rewrite Heqd'. rewrite nth_error_app. cbv [dag.lookup] in H2. rewrite Heqd' in H2. rewrite nth_error_app in H2.
+    destruct (lt_dec _ _) eqn: E.
+    + destruct (nth_error _ _) as [thing|] eqn:E'; try apply I. cbv [in_bounds]. destruct (snd thing) as [ [min max] |] eqn:Erange; try apply I.
+      assert (Forall (N.lt (N.of_nat (Datatypes.length d))) args0).
+
+
+
+
+
+ apply H with (G := G). Check ERef. apply ERef with (op := op0) (args := args0) (args' := args'). assumption. Print dag.ok.   simpl in Heqd'. cbv [dag.lookup] in H2. cbv [dag.merge_node] in H2. destruct (dag.reverse_lookup _ _) as [i_|] eqn:E'.
+  - simpl in H2. assert (dag.lookup cbv [dag.merge_node] in *. try rewrite E' in *. 
+ destruct (nth_error _ _) as [thing|] eqn:E; try apply I.
+  simpl in H2.
+
+ Print dag.merge_node.
+  remember (ExprRef i) as e. generalize dependent i. induction H0. induction H0.
+  - Check interp_bound_node.
+    intros. symmetry in Heqe. inv Heqe. Check interp_bound_node.
+    destruct (nth_error _ _) as [node|] eqn:E; try apply I. Check interp_bound_node.
+    
+    Search dag.lookup.
+  cbv [dag.merge_node]. inv H0. Check interp_bound_node. destruct (dag.reverse_lookup d (o, args)) as [i'|].
+  - simpl. apply H. apply H0.
+  - simpl in *. inv H0. cbv [dag.lookup] in H2. rewrite nth_error_app in H2.
+    cbv [dag.lookup_bounds]. rewrite nth_error_app.
+    destruct (lt_dec (N.to_nat i) (Datatypes.length d)).
+    + destruct (nth_error d (N.to_nat i)) as [thing|].
+      -- simpl in H2. *)
+
+(* cbv [in_bounds dag.lookup_bounds] in H0. rewrite nth_error_app in H0.
+    destruct (lt_dec (N.to_nat i) (Datatypes.length d)).
+    +  *)
 
 Lemma eval_merge_node {descr descr' descr'' descr'''} :
   forall G d, gensym_dag_ok G d ->
@@ -1496,7 +2184,7 @@ Lemma eval_merge_node {descr descr' descr'' descr'''} :
   gensym_dag_ok G (snd (@merge_node descr'' e d)) /\
   forall i e', eval G d i e' -> eval G (snd (@merge_node descr''' e d)) i e'.
 Proof using Type.
-  intros.
+  intros. destruct H as [H H'].
   cbv beta delta [merge_node].
   inversion H0; subst.
   cbv [gensym_dag_ok dag_ok] in *; destruct_head'_and.
@@ -1505,6 +2193,7 @@ Proof using Type.
   all: eauto using Forall2_weaken, eval_weaken_merge_node.
   all: try now apply gensym_ok_merge_node.
   { now rewrite dag.lookup_merge_node' by assumption. }
+  { apply merge_node_bounds_ok with (ctx := G); repeat (try split; try assumption). }
   { apply @dag.merge_node_all_nodes_ok; try assumption.
     cbv [e node_ok]; intros; inversion_pair; subst; cbn [interp_op] in *.
     break_innermost_match_hyps; inversion_option; subst.
@@ -1549,9 +2238,6 @@ Fixpoint list_of_addends (d : dag) (f : nat) (s : OperationSize) (i : idx) : lis
   end.
 
 Local Open Scope Z_scope.
-
-Lemma Z_land_ones' : forall (s : N) (a : Z), Z.land a (Z.ones (Z.of_N s)) = (a mod 2 ^ Z.of_N s)%Z.
-Proof. intros. assert (E: Z.le 0 (Z.of_N s)) by lia. auto using Z.land_ones. Qed.
 
 Lemma break_addZ_small : forall l1 l2,
   (fold_right Z.add 0 l1) + (fold_right Z.add 0 l2) = fold_right Z.add 0 (l1 ++ l2).
@@ -2730,6 +3416,263 @@ End AddcarryManipulation.
 
 Import AddcarryManipulation.
 
+Definition is_power_of_2 bound :=
+  if fst bound =? snd bound then
+    2^(Z.log2 (fst bound)) =? fst bound
+  else false.
+
+Definition left_shift d i :=
+  match dag.lookup_bounds d i with
+  | Some bounds => if (fst bounds =? snd bounds) && (2^(Z.log2 (fst bounds)) =? fst bounds) then
+    Z.log2 (fst bounds) else 0
+  | None => 0
+  end.
+
+Lemma left_shifted ctx d i n :
+  bounds_ok d ->
+  eval ctx d (ExprRef i) n ->
+  ((2 ^ (left_shift d i)) | n)%Z.
+Proof.
+  intros H_bounds H. cbv [left_shift]. cbv [bounds_ok] in H_bounds.
+  apply H_bounds in H. clear H_bounds. destruct (dag.lookup_bounds d i) as [ [min max]|] eqn:E1.
+  - simpl in *. destruct (min =? max) eqn:E2.
+    + destruct (2 ^ Z.log2 min =? min) eqn:E3.
+      -- apply Z.eqb_eq in E2. apply Z.eqb_eq in E3. subst. simpl. replace n with max by lia. rewrite E3.
+         exists 1. lia.
+      -- exists n. simpl. lia.
+    + exists n. simpl. lia.
+  - exists n. simpl. lia.
+Qed.
+
+Lemma left_shift_nonneg d i :
+  0 <= left_shift d i.
+Proof.
+  cbv [left_shift]. destruct (dag.lookup_bounds d i) as [bounds|]; try lia. destruct (_ && _); try lia. apply Z.log2_nonneg.
+Qed.
+
+Definition left_shifts (d : dag) (i : idx) :=
+  match dag.lookup d i with
+  | Some ((mul _ | mulZ), args) =>
+    fold_right Z.add 0 (map (left_shift d) args)
+  | _ => 0
+  end.
+
+Lemma abs_mod_0 a b :
+  (Z.abs a) mod (Z.abs b) = 0 ->
+  a mod b = 0.
+Proof.
+  destruct (b =? 0) eqn:E.
+  - apply Z.eqb_eq in E. subst. intros. rewrite Zmod_0_r in *. rewrite <- Z.abs_0_iff. apply H.
+  - intros. apply Z.eqb_neq in E. remember E as E'; clear HeqE'.
+    apply Z.rem_mod with (a := a) in E. rewrite H in E. apply Z.rem_mod_eq_0 with (a := a) in E'. rewrite <- E'.
+    lia.
+Qed.
+
+Lemma divide_mod a e b e' :
+  (a ^ e | b)%Z ->
+  (a ^ e | b mod (a ^ e'))%Z.
+Proof.
+  intros. destruct (0 <=? e') eqn:E0.
+  - apply Z.leb_le in E0. destruct (b =? 0) eqn:E0'. 
+    + apply Z.eqb_eq in E0'. subst. rewrite Zmod_0_l. exists 0. lia. 
+    + apply Z.eqb_neq in E0'. destruct (0 <=? e) eqn:E1. 
+      -- apply Z.leb_le in E1. destruct (e <=? e') eqn:E2.
+        ++ apply Z.leb_le in E2. apply Z.divide_add_cancel_r with (m := a ^ e' * (b / a ^ e')).
+          --- exists (a ^ (e' - e) * (b / a ^ e')). replace (a ^ e') with (a ^ e * a ^ (e' - e)); try lia.
+         rewrite <- Z.pow_add_r; try lia. f_equal. lia.
+          --- rewrite <- Z_div_mod_eq_full. apply H.
+        ++ apply Z.leb_nle in E2. replace (b mod a ^ e') with 0.
+          --- exists 0. lia.
+          --- symmetry. apply abs_mod_0. rewrite Znumtheory.Zmod_div_mod with (m := Z.abs b).
+            +++ rewrite Z_mod_same_full. rewrite Zmod_0_l. reflexivity.
+            +++ remember (Z.abs_nonneg (a ^ e')) as H1; clear HeqH1. assert (a ^ e' <> 0).
+              ---- intros H'. rewrite Z.pow_eq_0_iff in H'. destruct H' as [H'|H'].
+                ++++ lia.
+                ++++ assert (H'': e <> 0) by lia. destruct H' as [_ H']. subst. apply Z.pow_0_l' in H''.
+                     rewrite H'' in H. destruct H as [x H]. lia.
+              ---- rewrite <- Z.abs_0_iff in H0. lia.
+            +++ remember (Z.abs_nonneg b) as H1; clear HeqH1. rewrite <- Z.abs_0_iff in E0'. lia.
+            +++ rewrite Z.divide_abs_l. rewrite Z.divide_abs_r.
+                replace e with (e' + (e - e')) in H by lia. rewrite Z.pow_add_r in H by lia.
+                destruct H as [x H]. exists (x * a ^ (e - e')). lia.
+      -- apply Z.leb_nle in E1. replace (a ^ e) with 0 in H.
+              ---- destruct H as [x H].  lia.
+              ---- symmetry. apply Z.pow_neg_r. lia.
+  - apply Z.leb_nle in E0. replace (a ^ e') with 0. 
+    + rewrite Zmod_0_r. assumption. 
+    + symmetry. apply Z.pow_neg_r. lia.
+Qed.
+
+Check Forall.
+
+Lemma sum_nonneg l :
+  Forall (fun x => 0 <= x) l ->
+  0 <= fold_right Z.add 0 l.
+Proof.
+  induction l as [|x l' IHl'].
+  - intros. simpl. lia.
+  - intros. inv H. apply IHl' in H3. simpl. lia.
+Qed.
+
+Lemma exp_sum a l :
+  Forall (fun x => 0 <= x) l ->
+  a ^ fold_right Z.add 0 l = fold_right Z.mul 1 (map (fun x => a ^ x) l).
+Proof.
+  intros. induction l as [| x l' IHl'].
+  - simpl. reflexivity.
+  - simpl. inv H. remember (sum_nonneg _ H3) as H3'; clear HeqH3'. rewrite Z.pow_add_r by assumption.
+    apply IHl' in H3. rewrite H3. reflexivity.
+Qed.
+
+Lemma product_divide l1 l2 :
+  Forall2 (fun a b => Z.divide a b) l1 l2 ->
+  (fold_right Z.mul 1 l1 | fold_right Z.mul 1 l2).
+Proof.
+  generalize dependent l2. induction l1 as [|x l1' IHl1'].
+  - intros. inv H. simpl. exists 1. lia.
+  - intros. inv H. simpl. apply IHl1' in H4. destruct H2 as [x1 H2]. destruct H4 as [x2 H4]. exists (x2 * x1). lia.
+Qed.
+
+Lemma lefts_shifted ctx d i n :
+  bounds_ok d ->
+  eval ctx d (ExprRef i) n ->
+  (2^(left_shifts d i) | n)%Z.
+Proof.
+  intros H_bounds H. cbv [left_shifts].
+  destruct (dag.lookup d i) as [ [o args]|] eqn:E.
+  - inv H. rewrite H1 in E. inv E.
+    assert (H': (2 ^ fold_right Z.add 0 (map (left_shift d) args) | fold_right Z.mul 1 args')).
+    + assert (H4: Forall (fun x => 0 <= x) (map (left_shift d) args)).
+      { clear H1 H2. induction args as [|arg args1 IHargs1].
+        - constructor.
+        - constructor.
+          + apply left_shift_nonneg.
+          + apply IHargs1.
+      }
+      rewrite (exp_sum _ _ H4). clear H4. Check map_map. rewrite map_map. apply product_divide. clear H1 H3. generalize dependent args'.
+      induction args as [| arg args1 IHargs1].
+      -- intros. inv H2. constructor.
+      -- intros. inv H2. constructor.
+        ++ apply left_shifted with (ctx := ctx); assumption.
+        ++ apply IHargs1. assumption.
+    + destruct o; try (exists n; subst; lia).
+      -- inv H3. rewrite Z_land_ones'. apply divide_mod. apply H'.
+      -- inv H3. apply H'.
+  - exists n. lia.
+Qed.
+
+Definition or_is_add (d : dag) (args : list idx) : bool :=
+  match args with
+  | [arg1; arg2] =>
+    match dag.lookup_bounds d arg1 with
+    | Some bounds => if subset bounds (0, 2 ^ left_shifts d arg2 - 1) then true else
+      match dag.lookup_bounds d arg2 with
+      | Some bounds => if subset bounds (0, 2 ^ left_shifts d arg1 - 1) then true else false
+      | _ => false
+      end
+    | None => match dag.lookup_bounds d arg2 with
+              | Some bounds => if subset bounds (0, 2 ^ left_shifts d arg1 - 1) then true else false
+              | _ => false
+              end
+    end
+  | _ => false
+  end.
+
+Print interp_op.
+
+Lemma or_is_add_arith a b x :
+  (2 ^ x | a) ->
+  0 <= b < 2 ^ x ->
+  Z.lor a b = Z.add a b.
+Proof.
+  intros. destruct (0 <=? x) eqn:E.
+  - apply Z.leb_le in E. apply Z.or_to_plus. rewrite <- (Z.land_ones_low_alt b x); try lia.
+    rewrite (Z.land_comm b). rewrite Z.land_assoc. rewrite Z.land_ones; try assumption.
+      rewrite Znumtheory.Zdivide_mod by assumption. apply Z.land_0_l.
+  - apply Z.leb_nle in E. Search (_ ^ _ = 0). rewrite Z.pow_neg_r in H0 by lia. lia.
+Qed.
+
+Lemma subset_bounds bounds1 bounds2 :
+  subset bounds1 bounds2 = true ->
+  fst bounds2 <= fst bounds1 /\ snd bounds1 <= snd bounds2.
+Proof.
+  intros. cbv [subset] in H. apply andb_true_iff in H. destruct H as [H1 H2]. apply Z.leb_le in H1. apply Z.leb_le in H2.
+  split; assumption.
+Qed.
+
+Lemma eval_orZ_is_addZ d args ctx n :
+  bounds_ok d ->
+  or_is_add d args = true ->
+  eval ctx d (ExprApp (orZ, map ExprRef args)) n ->
+  eval ctx d (ExprApp (addZ, map ExprRef args)) n.
+Proof.
+  intros. cbv [or_is_add] in H0. destruct args as [| arg1 [| arg2 [| args'] ] ]; try discriminate H0.
+  inv H1. remember H4 as H5; clear HeqH5. inv H4. inv H8. inv H9. inv H6. rename y into arg1'. rename y0 into arg2'.
+  Print bounds_ok. remember (H _ _ _ H3) as H3'. remember (H _ _ _ H4) as H4'.
+  remember (lefts_shifted _ _ _ _ H H3) as H3''. remember (lefts_shifted _ _ _ _ H H4) as H4''. clear HeqH3' HeqH4' HeqH3'' HeqH4''.
+  apply EApp with (args' := [arg1'; arg2']); try assumption. simpl. f_equal. rewrite Z.add_0_r. rewrite Z.lor_0_r.
+  destruct (dag.lookup_bounds d arg1) as [bounds|] eqn:E1.
+  - destruct (subset bounds (0, 2 ^ left_shifts d arg2 - 1)) eqn:E2.
+    + symmetry. rewrite Z.lor_comm. rewrite Z.add_comm. apply or_is_add_arith with (x := left_shifts d arg2). 
+      -- apply H4''.
+      -- apply subset_bounds in E2. simpl in H3'. destruct bounds as [min max]. simpl in *. lia.
+    + destruct (dag.lookup_bounds d arg2) eqn:E3.
+      -- destruct (subset p _) eqn:E4.
+        ++ clear H0. symmetry. apply or_is_add_arith with (x := left_shifts d arg1).
+          --- apply H3''.
+          --- apply subset_bounds in E4. simpl in H4'. destruct p as [min max]. cbv [subset] in E4. simpl in *. lia.
+        ++ discriminate H0.
+      -- discriminate H0.
+  - destruct (dag.lookup_bounds d arg2) as [bounds|] eqn:E2.
+    + destruct (subset bounds (0, 2 ^ left_shifts d arg1 - 1)) eqn:E3.
+      -- clear H0. symmetry. apply or_is_add_arith with (x := left_shifts d arg1).
+        ++ apply H3''.
+        ++ apply subset_bounds in E3. simpl in H4'. destruct bounds as [min max]. simpl in *. lia.
+      -- discriminate H0.
+    + discriminate H0.
+Qed.
+
+Check adds_to_addZ.
+
+Lemma ors_to_orZ ctx d s args n :
+  eval ctx d (ExprApp (or s, args)) n ->
+  exists m,
+  n = m mod (2 ^ Z.of_N s) /\
+  eval ctx d (ExprApp (orZ, args)) m.
+Proof.
+  intros. inv H. exists (fold_right Z.lor 0 args'). inv H4. split.
+  - rewrite Z_land_ones'. reflexivity.
+  - apply EApp with (args' := args').
+    + apply H2.
+    + simpl. reflexivity.
+Qed.
+
+Lemma eval_ors_is_adds d args ctx n s :
+  bounds_ok d ->
+  or_is_add d args = true ->
+  eval ctx d (ExprApp (or s, map ExprRef args)) n ->
+  eval ctx d (ExprApp (add s, map ExprRef args)) n.
+Proof.
+  intros. apply ors_to_orZ in H1. destruct H1 as [m [H1 H2] ]. subst. apply addZ_to_adds. apply eval_orZ_is_addZ; assumption.
+Qed.
+
+Definition new_op (d : dag) (o : op) (args : list idx) : op :=
+  match o with
+  | or s => if or_is_add d args then add s else or s
+  | orZ => if or_is_add d args then addZ else orZ
+  | _ => o
+  end.
+
+Lemma eval_new_op ctx d o args n :
+  bounds_ok d ->
+  eval ctx d (ExprApp (o, map ExprRef args)) n ->
+  eval ctx d (ExprApp (new_op d o args, map ExprRef args)) n.
+Proof.
+  intros. cbv [new_op]. destruct o; try apply H0.
+  - destruct (or_is_add _ _) eqn:E; try apply H0. apply eval_ors_is_adds; assumption.
+  - destruct (or_is_add _ _) eqn:E; try apply H0. apply eval_orZ_is_addZ; assumption.
+Qed.
+
 Fixpoint merge {descr : description} (e : expr) (d : dag) : idx * dag :=
   match e with
   | ExprRef i => (i, d)
@@ -2742,7 +3685,8 @@ Fixpoint merge {descr : description} (e : expr) (d : dag) : idx * dag :=
     let idxs := if commutative op
                 then N.sort (fst idxs_d')
                 else (fst idxs_d') in
-    merge_node (op, idxs) (snd idxs_d')
+    let op' := new_op (snd idxs_d') op idxs in
+    merge_node (op', idxs) (snd idxs_d')
   end.
 
 Lemma eval_merge {descr:description} G :
@@ -2791,12 +3735,16 @@ Proof using Type.
         simpl. destruct H'' as [H1 [H2 H3] ]. auto.
       - subst. auto.
     }
-    clear H_ok0 H_eval0 H'' Heqidxs_d' H. destruct H''' as [H_ok' [H' H_eval'] ]. destruct (commutative o) eqn:Eo.
+    clear H_ok0 H_eval0 H'' Heqidxs_d' H. destruct H''' as [H_ok' [H' H_eval'] ].
+    remember H_ok' as bounds_ok'; clear Heqbounds_ok'. destruct bounds_ok' as [_ [bounds_ok' _] ].
+    destruct (commutative o) eqn:Eo.
     + assert (Hperm: Permutation (map ExprRef (fst idxs_d')) (map ExprRef (N.sort (fst idxs_d')))).
       { apply Permutation_map. apply N.Sort.Permuted_sort. }
-      apply (eval_permute_commutative _ _ _ _ _ _ Eo Hperm) in H'. clear Eo Hperm.
+      apply (eval_permute_commutative _ _ _ _ _ _ Eo Hperm) in H'.
+      apply (eval_new_op _ _ _ _ _ bounds_ok') in H'.
       apply (eval_merge_node _ _ H_ok') in H'. subst. destruct H' as [H1 [H2 H3] ]. auto.
-    + apply (eval_merge_node _ _ H_ok') in H'. subst. destruct H' as [H1 [H2 H3] ]. auto.
+    + apply (eval_new_op _ _ _ _ _ bounds_ok') in H'. apply (eval_merge_node _ _ H_ok') in H'. subst.
+      destruct H' as [H1 [H2 H3] ]. auto.
 Qed.
 
 Definition zconst s (z:Z) := const (Z.land z (Z.ones (Z.of_N s)))%Z.
@@ -3593,6 +4541,8 @@ Definition shift_to_mul :=
 Global Instance shift_to_mul_ok : Ok shift_to_mul.
 Proof. t; cbn in *; rewrite ?Z.shiftl_mul_pow2, ?Z.land_0_r by lia; repeat (lia + f_equal). Qed.
 
+Print op.
+
 (* o is like mul *)
 (* invariant: Forall2 (fun x '(y, z) => eval (o x i) matches eval (o y z)) input output *)
 Definition split_consts (o : op) (i : Z) : list expr -> list (expr * Z)
@@ -4214,8 +5164,9 @@ Global Instance show_flag_state : Show flag_state :=
 
 Global Instance show_lines_dag : ShowLines dag := (fun d:dag =>
   ["(*dag*)["]
-    ++List.map (fun '(i, v, descr) =>"(*"++show i ++"*) " ++ show v++";"
-                                         ++ (if dag.get_eager_description_always_show descr
+    ++List.map (fun '(i, v, descr, bounds) =>"(*"++show i ++"*) " ++ show v++";"
+                                         ++ "(((" ++ show bounds ++ ")))" ++ 
+                                            (if dag.get_eager_description_always_show descr
                                              then match dag.get_eager_description_description descr with
                                                   | Some descr => " " ++ String.Tab ++ "(*" ++ descr ++ "*)"
                                                   | None => ""
